theories/StaticApply.v
@@ -70,12 +70,13 @@ Definition remove_ret {V} {B} {Q : B -> Type} {A} : forall (v : V) b (m : Q b), 
 .
 
 Set Printing Universes.
-Definition apply_type_of (P : Type) :
+Set Use Unicoq.
+Program Definition apply_type_of (P : Type) :
   forall {T} (t : T),
                       M (sigT (funs_of (M P))) :=
   mfix f (T : _) : T -> M (sigT (funs_of (M P))) :=
-     mtmmatch T as T' return T' -> M (sigT (funs_of (M P))) with
-     | (M P : Type) =c> fun t => M.ret (existT _ [m:] t)
+     mtmmatch_prog T as T' return T' -> M (sigT (funs_of (M P))) with
+     | (M P : Type) =c> fun t => M.ret (existT (funs_of (M P)) [m:] t)
      | [? X F] (forall x : X, F x) =c>
         fun ft =>
           s <- M.fresh_binder_name ft;
